examples/cellio/CellioA.v
@@ -75,5 +75,5 @@ Module CellioA. Section CellioA.
 
   Variable ginv: Sk.t -> invspec.
   Variable GlobalStb: Sk.t -> string -> option fspec.
-  Definition t := Seal.sealing "ccr" (SMod.to_hmod ginv GlobalStb Mod).
+  Definition t := Seal.sealing CRIS (SMod.to_hmod ginv GlobalStb Mod).
 End CellioA. End CellioA.
