examples/cellio/MainI.v
@@ -37,6 +37,6 @@ Section MainI.
   |}
   .
 
-  Definition t := Seal.sealing "ccr" (PMod.to_hmod Mod).
+  Definition t := Seal.sealing CRIS (PMod.to_hmod Mod).
 
 End MainI. End MainI.
