examples/map/MapIAproof.v
@@ -14,14 +14,14 @@ Module MapIA. Section MapIA.
     etrans; cycle 1.
     { eapply main_adequacy. eapply MapIM.sim.
       instantiate (1:= const(to_stb MapMS.Stb)).
-      i. split; try refl. unfold MapMS.Stb. unseal "ccr". prove_nodup.
+      i. split; try refl. unfold MapMS.Stb. unseal CRIS. prove_nodup.
     }
     etrans; cycle 1.
     { eapply ctxr_frameR.
       rewrite -(hmod_addc_empty_l _ MapMS.InitCond).
       eapply ctxr_cond_frameR, main_adequacy, MapMA.sim; eauto.
       intros sk; split; try refl.
-      rewrite /MapMS.Stb; unseal "ccr"; prove_nodup.
+      rewrite /MapMS.Stb; unseal CRIS; prove_nodup.
     }
     refl.
   Qed.
