examples/ring/CtrlI.v
@@ -75,6 +75,6 @@ Module CtrlI. Section CtrlI.
   |}
   .
 
-  Definition t := Seal.sealing "ccr" (PMod.to_hmod Mod).
+  Definition t := Seal.sealing CRIS (PMod.to_hmod Mod).
 
 End CtrlI. End CtrlI. *)
