examples/scheduler/SchI.v
@@ -82,6 +82,6 @@ Module SchI. Section SchI.
     PMod.sk := SchSK.t;
   |}.
 
-  Definition t := Seal.sealing "ccr" (PMod.to_hmod Mod).
+  Definition t := Seal.sealing CRIS (PMod.to_hmod Mod).
 
 End SchI. End SchI.
